Veritas.SeqAux.fsti
@@ -247,6 +247,10 @@ val lemma_map_index (#a #b: Type) (f:a -> b) (s:seq a) (i:seq_index s):
         (ensures (f (index s i) == index (map f s) i))
         [SMTPat (index (map f s) i)]
 
+val lemma_map_prefix (#a #b: Type) (f:a -> b) (s:seq a) (i: seq_index s):
+  Lemma (requires True)
+        (ensures (map f (prefix s i) == prefix (map f s) i))
+
 val zip (#a #b: eqtype) (sa: seq a) (sb: seq b{length sb = length sa}):
   sab: seq (a * b){length sab = length sa}
 
